Update to use the newest FFI.fst interface
Update to use the newest FFI.fst interface

libs/ml/FFICallbacks.ml
@@ -3,12 +3,12 @@ external ocaml_send_tcp: callbacks -> string -> int = "ocaml_send_tcp"
 external ocaml_recv_tcp: callbacks -> string -> int = "ocaml_recv_tcp"
 
 (*module FFICallbacks = struct *)
-  let recv sock maxlen =
+  let recvcb sock maxlen =
       let str = Bytes.create maxlen in
       let recvlen = ocaml_recv_tcp sock str in
       if recvlen < 0 then 
-        (0, Platform.Bytes.empty_bytes)
+        (0, "")
       else
         let str = String.sub str 0 recvlen in
-        (1, Platform.Bytes.abytes str)
+        (1, str)
 (* end *)
